ulib/FStar.Monotonic.HyperStack.fst
@@ -4,14 +4,18 @@ open FStar.Preorder
 open FStar.Monotonic.HyperHeap
 module M  = FStar.Map
 module HH = FStar.Monotonic.HyperHeap
+module Set = FStar.Set
 
-let is_in (r:rid) (h:HH.t) = h `Map.contains` r
+(*+ Convenience predicates on rids +*)
+
+let is_in (r:rid) (h:HH.t) = h `contains` r
 
 let is_stack_region r = color r > 0
 let is_eternal_color c = c <= 0
 let is_eternal_region r  = is_eternal_color (color r)
 
-type sid = r:rid{is_stack_region r} //stack region ids
+(* stack region ids *)
+type sid = r:rid{is_stack_region r}
 
 let is_above r1 r2      = r1 `includes` r2
 let is_just_below r1 r2 = r1 `extends`  r2
@@ -19,30 +23,49 @@ let is_below r1 r2      = r2 `is_above` r1
 let is_strictly_below r1 r2 = r1 `is_below` r2 && r1<>r2
 let is_strictly_above r1 r2 = r1 `is_above` r2 && r1<>r2
 
+
+(*+ Definition of the HyperStack memory model (mem) +*)
+
 let downward_closed (h:HH.t) =
-  forall (r:rid). r `is_in` h  //for any region in the memory
-        ==> (r==HH.root    //either is the root
-	    \/ (forall (s:rid). r `is_above` s  //or, any region beneath it
-			  /\ s `is_in` h   //that is also in the memory
-		     ==> (is_stack_region r == is_stack_region s))) //must be of the same flavor as itself
+  (* for any region in the memory *)
+  forall (r:rid). r `is_in` h ==> (
+    (* either is the root *)
+    r == HH.root
+    (* or, any region beneath it that is also in the memory *)
+	  \/ (forall (s:rid). r `is_above` s /\ s `is_in` h ==>
+        (* must be of the same flavor as itself *)
+		    is_stack_region r == is_stack_region s))
 
 let is_tip (tip:HH.rid) (h:HH.t) =
-  (is_stack_region tip \/ tip==HH.root)                                  //the tip is a stack region, or the root
-  /\ tip `is_in` h                                                      //the tip is active
-  /\ (forall (r:sid). r `is_in` h <==> r `is_above` tip)                      //any other sid activation is a above (or equal to) the tip
+  (* the tip is a stack region, or the root *)
+  (is_stack_region tip \/ tip==HH.root)
+  (* the tip is activated *)
+  /\ tip `is_in` h
+  (* any other sid activation is above (or equal to) the tip *)
+  /\ (forall (r:sid). r `is_in` h <==> r `is_above` tip)
 
-let hh = h:HH.t{HH.root `is_in` h /\ HH.map_invariant h /\ downward_closed h}        //the memory itself, always contains the root region, and the parent of any active region is active
+let eternal_is_live (h:HH.t) =
+  (* Any eternal region contained in the heap must be live *)
+  forall (r:HH.rid). is_eternal_region r /\ Map.contains h r ==> (Map.sel h r).live
+
+(* the memory itself, always contains the root region, and the parent of any active region is active *)
+let hh = h:HH.t{HH.root `is_in` h /\ HH.map_invariant h /\ downward_closed h /\ eternal_is_live h}
 
 noeq type mem =
-  | HS : h:hh
-       -> tip:rid{tip `is_tip` h}                                                   //the id of the current top-most region
-       -> mem
+  | HS :
+    h:hh ->
+    (* the id of the current top-most region *)
+    tip:rid{tip `is_tip` h} ->
+    mem
 
 let empty_mem (m:HH.t) =
   let empty_map = Map.restrict (Set.empty) m in
-  let h = Map.upd empty_map HH.root Heap.emp in
+  let h = Map.upd empty_map HH.root (H true Heap.emp) in
   let tip = HH.root in
   HS h tip
+
+
+(*+ Tests +*)
 
 let test0 (m:mem) (r:rid{r `is_above` m.tip}) =
     assert (r `is_in` m.h)
@@ -65,35 +88,37 @@ let test4 (m:mem) (r:rid{r =!= HH.root /\ is_eternal_region r /\ r `is_above` m.
   : Lemma (~ (r `is_in` m.h))
   = ()
 
-let eternal_region_does_not_overlap_with_tip (m:mem) (r:rid{is_eternal_region r /\ not (HH.disjoint r m.tip) /\ r=!=HH.root /\ is_stack_region m.tip})
-  : Lemma (requires True)
+let eternal_region_does_not_overlap_with_tip (m:mem) (r:rid)
+  : Lemma (requires (
+      is_eternal_region r /\
+      not (HH.disjoint r m.tip) /\
+      r =!= HH.root /\
+      is_stack_region m.tip))
 	  (ensures (~ (r `is_in` m.h)))
-  = root_has_color_zero()
+= root_has_color_zero()
 
 let poppable m = m.tip =!= HH.root
-
-let remove_elt (#a:eqtype) (s:Set.set a) (x:a) = Set.intersect s (Set.complement (Set.singleton x))
 
 let popped m0 m1 =
   poppable m0
   /\ HH.parent m0.tip == m1.tip
-  /\ Set.equal (Map.domain m1.h) (remove_elt (Map.domain m0.h) m0.tip)
-  /\ Map.equal m1.h (Map.restrict (Map.domain m1.h) m0.h)
+  /\ Set.equal (Map.domain m1.h) (Map.domain m0.h)
+  /\ (let common_domain = Map.domain m0.h `Set.remove_elt` m0.tip in
+    Map.equal (Map.restrict common_domain m1.h) (Map.restrict common_domain m0.h)
+    /\ ~(Map.sel m1.h m0.tip).live)
 
-let pop (m0:mem{poppable m0}) : Tot (m1:mem{popped m0 m1}) =
-  root_has_color_zero();
-  let dom = remove_elt (Map.domain m0.h) m0.tip in
-  let h0 = m0.h in
-  let h1 = Map.restrict dom m0.h in
-  let tip0 = m0.tip in
-  let tip1 = HH.parent tip0 in
-  assert (forall (r:sid). Map.contains h1 r ==>
-  	    (forall (s:sid). includes s r ==> Map.contains h1 s));
-  let m1 = HS h1 tip1 in
-  assert (Set.equal (Map.domain m1.h) (remove_elt (Map.domain m0.h) m0.tip)) ;
-  assert (Map.equal m1.h (Map.restrict (Map.domain m1.h) m0.h)) ;
-  m1
+let pop (m0:mem{poppable m0}) : Tot (m1:mem) =
+  let v = H false (m0.h `HH.at` m0.tip) in
+  let h1 = Map.upd m0.h m0.tip v in
+  let tip1 = HH.parent m0.tip in
+  assert (forall (r:sid). r `is_in` h1 <==> r `is_above` tip1) ;
+  HS h1 tip1
 
+let lemma_pop_is_popped (m0:mem{poppable m0})
+  : Lemma (popped m0 (pop m0))
+= let m1 = pop m0 in
+  Map.lemma_DomRestrUpd_equal m0.h m0.tip (Map.sel m1.h m0.tip) ;
+  assert (Set.equal (Map.domain m1.h) (Map.domain m0.h))
 
 //A (reference a) may reside in the stack or heap, and may be manually managed
 noeq type mreference (a:Type) (rel:preorder a) =
@@ -102,11 +127,11 @@ noeq type mreference (a:Type) (rel:preorder a) =
 let is_mm (#a:Type) (#rel:preorder a) (r:mreference a rel) :GTot bool = HH.is_mm r.ref
 
 //adding (not s.mm) to stackref and ref so as to keep their semantics as is
-let mstackref (a:Type) (rel:preorder a) = s:mreference a rel{ is_stack_region s.id && not (is_mm s) }
-let mref (a:Type) (rel:preorder a) = s:mreference a rel{is_eternal_region s.id && not (is_mm s)}
+let mstackref (a:Type) (rel:preorder a) = s:mreference a rel{ is_stack_region s.id /\ not (is_mm s) }
+let mref (a:Type) (rel:preorder a) = s:mreference a rel{is_eternal_region s.id /\ not (is_mm s)}
 
-let mmmstackref (a:Type) (rel:preorder a) = s:mreference a rel{is_stack_region s.id && is_mm s }
-let mmmref (a:Type) (rel:preorder a) = s:mreference a rel{is_eternal_region s.id && is_mm s}
+let mmmstackref (a:Type) (rel:preorder a) = s:mreference a rel{is_stack_region s.id /\ is_mm s }
+let mmmref (a:Type) (rel:preorder a) = s:mreference a rel{is_eternal_region s.id /\ is_mm s}
 
 (*
  * The Map.contains conjunct is necessary to prove that upd
@@ -116,7 +141,7 @@ let mmmref (a:Type) (rel:preorder a) = s:mreference a rel{is_eternal_region s.id
  *)
 let live_region (m:mem) (i:rid) =
   (is_eternal_region i \/ i `is_above` m.tip)
-  /\ Map.contains m.h i
+  /\ m.h `HH.contains` i
 
 (*
  * AR: adding a weaker version of live_region that could be
@@ -135,7 +160,7 @@ let unused_in (#a:Type) (#rel:preorder a) (r:mreference a rel) (h:mem) =
 
 private val weak_live_region_implies_eternal_or_in_map: r:rid -> m:mem -> Lemma
   (requires (weak_live_region m r))
-  (ensures (is_eternal_region r \/ Map.contains m.h r))
+  (ensures (is_eternal_region r \/ m.h `HH.contains` r))
 let weak_live_region_implies_eternal_or_in_map r m = ()
 
 (*
@@ -146,23 +171,25 @@ let weak_live_region_implies_eternal_or_in_map r m = ()
  *)
 let weak_contains (#a:Type) (#rel:preorder a) (m:mem) (s:mreference a rel) =
   weak_live_region m s.id /\
-  (if is_mm s then HH.weak_contains_ref s.ref m.h else True)
+  (if is_mm s then m.h `HH.weak_contains_ref` s.ref else True)
 
+(* KM : should we add the tot variants here too ? *)
 (*
  * AR: why is this not enforcing live_region ?
  *)
 let sel (#a:Type) (#rel:preorder a) (m:mem) (s:mreference a rel)
   : GTot a
-  = m.h.[s.ref]
+= m.h.[s.ref]
 
 let upd (#a:Type) (#rel:preorder a) (m:mem) (s:mreference a rel{live_region m s.id}) (v:a{rel (sel m s) v})
   : GTot mem
-  = HS (m.h.[s.ref] <- v) m.tip
+= HS (m.h.[s.ref] <- v) m.tip
 
 let equal_domains (m0:mem) (m1:mem) =
   m0.tip == m1.tip
   /\ Set.equal (Map.domain m0.h) (Map.domain m1.h)
-  /\ (forall r. Map.contains m0.h r ==> Heap.equal_dom (Map.sel m0.h r) (Map.sel m1.h r))
+  /\ (forall r. Map.contains m0.h r ==> (Map.sel m0.h r).live == (Map.sel m1.h r).live)
+  /\ (forall r. r `is_in` m0.h ==> Heap.equal_dom (m0.h `HH.at` r) (m1.h `HH.at` r))
 
 let lemma_equal_domains_trans (m0:mem) (m1:mem) (m2:mem) : Lemma
   (requires (equal_domains m0 m1 /\ equal_domains m1 m2))
@@ -171,8 +198,8 @@ let lemma_equal_domains_trans (m0:mem) (m1:mem) (m2:mem) : Lemma
   = ()
 
 let equal_stack_domains (m0:mem) (m1:mem) =
-  m0.tip = m1.tip
-  /\ (forall r. (is_stack_region r /\ r `is_above` m0.tip) ==> Heap.equal_dom (Map.sel m0.h r) (Map.sel m1.h r))
+  m0.tip == m1.tip
+  /\ (forall r. (is_stack_region r /\ r `is_above` m0.tip) ==> Heap.equal_dom (m0.h `HH.at` r) (m1.h `HH.at` r))
 
 let lemma_equal_stack_domains_trans (m0:mem) (m1:mem) (m2:mem) : Lemma
   (requires (equal_stack_domains m0 m1 /\ equal_stack_domains m1 m2))
@@ -182,32 +209,29 @@ let lemma_equal_stack_domains_trans (m0:mem) (m1:mem) (m2:mem) : Lemma
 
 let modifies (s:Set.set rid) (m0:mem) (m1:mem) =
   HH.modifies_just s m0.h m1.h
-  /\ m0.tip=m1.tip
+  /\ m0.tip == m1.tip
 
 let modifies_transitively (s:Set.set rid) (m0:mem) (m1:mem) =
   HH.modifies s m0.h m1.h
-  /\ m0.tip=m1.tip
+  /\ m0.tip == m1.tip
 
 let heap_only (m0:mem) =
   m0.tip == HH.root
 
-let top_frame (m:mem) = Map.sel m.h m.tip
+let top_frame (m:mem) = m.h `HH.at` m.tip
 
 let fresh_frame (m0:mem) (m1:mem) =
   not (Map.contains m0.h m1.tip)
   /\ HH.parent m1.tip == m0.tip
-  /\ m1.h == Map.upd m0.h m1.tip Heap.emp
+  /\ m1.h `Map.equal` Map.upd m0.h m1.tip HH.(H true Heap.emp)
 
-let modifies_drop_tip (m0:mem) (m1:mem) (m2:mem) (s:Set.set rid)
-    : Lemma (fresh_frame m0 m1 /\
-	     modifies_transitively (Set.union s (Set.singleton m1.tip)) m1 m2 ==>
-	     modifies_transitively s m0 (pop m2))
-    = ()
+(* TODO (KM) don't understand how this lemma is valid, dropping it temporarily since it does not seem to be used in this file *)
+(* let modifies_drop_tip (m0:mem) (m1:mem) (m2:mem) (s:Set.set rid) *)
+(*   : Lemma (fresh_frame m0 m1 /\ *)
+(*       modifies_transitively (s `Set.add_elt` m1.tip) m1 m2 ==> *)
+(*       modifies_transitively s m0 (pop m2)) *)
+(*   = () *)
 
-let lemma_pop_is_popped (m0:mem{poppable m0})
-  : Lemma (popped m0 (pop m0))
-  = let m1 = pop m0 in
-    assert (Set.equal (Map.domain m1.h) (remove_elt (Map.domain m0.h) m0.tip))
 
 type s_mref (i:rid) (a:Type) (rel:preorder a) = s:mreference a rel{s.id == i}
 
@@ -259,7 +283,7 @@ let contains_implies_weak_contains (#a:Type) (#rel:preorder a) (h:mem) (x:mrefer
   = ()
 
 noeq type some_ref =
-| Ref : #a:Type0 -> #rel:preorder a -> mreference a rel -> some_ref
+  | Ref : #a:Type0 -> #rel:preorder a -> mreference a rel -> some_ref
 
 let some_refs = list some_ref
 
